theories/tutorial/demo_reflection.v
@@ -1,69 +1,187 @@
-Require Import Arith ZArith Psatz List.
+
+(**
+   This example covers reifying an expression into a syntax tree.
+
+   This operation cannot be performed in Gallina itself, hence a meta
+   language is needed. Typical approaches are core written in ML, Ltac,
+   type class resolution.
+
+*)
+
+Require Arith ZArith Psatz List ssreflect.
+From elpi Require Import elpi.
+
+
+
+Import Arith ZArith Psatz List ssreflect.
+
+Module MonoidTheory.
+
+(* The syntax of terms *)
+Inductive lang :=
+| var (i : nat)        (* De Bruijn index, i-th variable in the context *)
+| zero : lang          (* Neutral element *)
+| add (x y : lang).    (* binary operation *)
+
+(* Interpretation to Z *)
+Fixpoint interp T (e : T) (op : T -> T -> T) (gamma : list T) (t : lang) : T :=
+match t with
+| var v => nth v gamma e
+  | zero => e
+  | add x y => op (interp T e op gamma x) (interp T e op gamma y)
+  end.
+ 
+
+ (* normalization of parentheses and units *)
+ Fixpoint normAx t1 acc :=
+   match t1 with
+   | add t1 t2 => normAx t1 (normAx t2 acc)
+   | _ => add t1 acc
+   end.
+ Fixpoint normA t :=
+   match t with
+   | add s1 s2 => normAx s1 (normA s2)
+   | _ => t
+   end.
+ Fixpoint norm1 t :=
+  match t with
+  | var _ => t
+  | zero => t
+  | add t1 t2 =>
+     match norm1 t1 with
+     | zero => norm1 t2
+     | t1 =>
+         match norm1 t2 with
+         | zero => t1
+         | t2 => add t1 t2
+         end
+     end
+  end.
+ Definition norm t := normA (norm1 t).
+
+  (* Correctness theorem *)
+ Section assoc_reflection_proofs.
+ Variable T : Type.
+ Variable unit : T.
+ Variable op : T -> T -> T.
+ Hypothesis op_assoc : forall a b c, op a (op b c) = op (op a b) c.
+ Hypothesis unit_l : forall a, op unit a = a.
+ Hypothesis unit_r : forall a, op a unit = a.
+
+ (*
+Lemma norm1_add {t1 t2} : norm1 (add t1 t2) = 
+                     if norm1 t1 is zero then norm1 t2 else
+                     if norm1 t2 is zero then norm1 t1 else
+                     add (norm1 t1) (norm1 t2).
+Proof. by case E1: (norm1 t1); case E2: (norm1 t2); rewrite /= ?E1 ?E2. Qed.
+
+Lemma norm_add {t1 t2} :
+  norm (add t1 t2) = if norm1 t1 is zero then normA (norm1 t2) else
+                     if norm1 t2 is zero then normA (norm1 t1) else
+                     normA (add (norm1 t1) (norm1 t2)).
+Proof. by rewrite /norm norm1_add; case E1: (norm1 t1); case E2: (norm1 t2). Qed.
+*)
+
+Lemma normAxA t1 t2 : normAx t1 (normA t2) = normA (add t1 t2).
+Proof. by []. Qed.
+
+Lemma normAx_add {t1 t2 s} : normAx t1 t2 = s -> exists s1 s2, s = add s1 s2.
+Proof.
+elim: t1 t2 s => /= [i||w1 H1 w2 H2] t2 s <-; try by do 2 eexists; reflexivity.
+by case E: (normAx _ _); case/H1: E => s1 [s2 ->]; do 2 eexists; reflexivity.
+Qed.
+
+Lemma norm1_zero {l t} : norm1 t = zero -> interp T unit op l t = unit.
+Proof.
+by elim: t => [||s1 + s2] //=; case E1: (norm1 s1); case E2: (norm1 s2) => //= -> // ->.
+Qed.
+
+Lemma norm_zero {l t} : norm t = zero -> interp T unit op l t = unit.
+Proof.
+rewrite /norm; case E: (norm1 t) => [||x y] //; first by rewrite (norm1_zero E).
+by move/normAx_add=> [] ? [].
+Qed.
+
+Lemma norm1_var {l t j} : norm1 t = var j -> interp T unit op l t = nth j l unit.
+Proof.
+elim: t => [i [->]||s1 + s2] //=; case E1: (norm1 s1); case E2: (norm1 s2) => //=.
+  by rewrite (norm1_zero E2) unit_r => + _ H => ->.
+by rewrite (norm1_zero E1) unit_l => _ + H => ->.
+Qed.
+
+Lemma norm_var {l t j} : norm t = var j -> interp T unit op l t = nth j l unit.
+Proof.
+rewrite /norm; case E: (norm1 t); rewrite /= ?(norm1_var E) //; first by move=> [->].
+by move/normAx_add=> [] ? [].
+Qed.
+
+Lemma norm1_add {l t s1 s2} : norm1 t = add s1 s2 -> interp T unit op l t = op (interp T unit op l s1) (interp T unit op l s2).
+Proof.
+elim: t s1 s2 => [i||w1 + w2 + s1 s2 E] //=; move: E => /=; case E1: (norm1 w1); case E2: (norm1 w2) => //=;
+  rewrite /= ?(norm1_zero E1) ?(norm1_zero E2) ?(norm1_var E1) ?(norm1_var E2) //= => -[<- <-] //=;
+  try move=> /(_ _ _ (refl_equal _)) <-;
+  try move=> + /(_ _ _ (refl_equal _)) <-;
+  rewrite ?unit_l ?unit_r //;
+  by move=> /(_ _ _ (refl_equal _)) <-.
+Qed.
+
+Lemma normAxP {l t1 t2} : interp T unit op l (normAx t1 t2) = op (interp T unit op l t1) (interp T unit op l t2).
+Proof. by elim: t1 t2 => [||s1 Hs1 s2 Hs2] t2 //=; rewrite Hs1 Hs2 !op_assoc. Qed.
+
+Lemma normAP {l} t : interp T unit op l (normA t) = interp T unit op l t.
+Proof. by elim: t => //= x Hx y Hy; rewrite normAxP Hy. Qed.
+
+Lemma norm_add {l t s1 s2} : norm t = add s1 s2 -> interp T unit op l t = op (interp T unit op l s1) (interp T unit op l s2).
+Proof.
+rewrite /norm; case E: (norm1 t) => [||x y]; rewrite //= (norm1_add E).
+elim: x y s1 s2 {E} => //= [????[<- <- //=]|???[<- <-]|x + y + w s1 s2]; rewrite ?normAP //= ?unit_l //.
+by rewrite normAxA -!op_assoc => ++ E => /(_ _ _ _ E) ->.
+Qed.
+
+Lemma normP_ l t1 t2 : norm t1 = norm t2 -> interp T unit op l t1 = interp T unit op l t2.
+Proof.
+case E: (norm t2) => [?||??] => [/norm_var|/norm_zero|/norm_add] ->.
+  by rewrite (norm_var E).
+  by rewrite (norm_zero E).
+by rewrite (norm_add E).
+Qed.
+
+End assoc_reflection_proofs.
+End MonoidTheory.
+
+Import MonoidTheory.
+
+Definition normP {T op zero l t1 t2} p1 p2 p3 H := @normP_ T op zero p1 p2 p3 l t1 t2 H.
 
 Open Scope Z_scope.
 
-Inductive lang := var (_ : nat) | add (_ _ : lang).
-
-Fixpoint interp (op : Z -> Z -> Z) (l : list Z) (t : lang) : Z :=
-  match t with
-  | var v => nth v l 0
-  | add x y => op (interp op l x) (interp op l y)
-  end.
-
-Fixpoint norm_aux t1 t2 : lang :=
-  match t1 with
-  | var x => add (var x) t2
-  | add t t' => norm_aux t (norm_aux t' t2)
-  end.
-
-Fixpoint norm t :=
-  match t with
-  | var x => t
-  | add t1 t2 => norm_aux t1 (norm t2)
-  end.
-
-Section assoc_reflection_proofs.
-
-Variable op : Z -> Z -> Z.
-
-Hypothesis op_assoc : forall a b c, op a (op b c) = op (op a b) c.
-
-Lemma norm_aux_c l t1 t2 :
-  interp op l (norm_aux t1 t2) = op (interp op l t1) (interp op l t2).
+Goal forall x y z t, (x + y) + (z + 0 + t) = x + (y + z) + t.
 Proof.
-revert t2; induction t1 as [i | t1 IH1 t2 IH2]; intros t3.
-  now auto.
-now simpl; rewrite IH1, IH2, op_assoc.
-Qed.
-
-Lemma norm_c l t :  interp op l t = interp op l (norm t).
-Proof.
-induction t as [i | t1 IH1 t2 IH2]; auto; simpl.
-now rewrite IH2, norm_aux_c.
-Qed.
-
-Lemma norm_c2 l t1 t2 : norm t1 = norm t2 -> interp op l t1 = interp op l t2.
-Proof. now intros nn; rewrite (norm_c _ t1), (norm_c _ t2); apply f_equal.  Qed.
-
-End assoc_reflection_proofs.
-
-Arguments norm_c2 {op}.
-
-Example axpypzpt x y z t : (x + y) + (z + t) = x + (y + z) + t.
-Proof.
-change (interp Z.add (x::y::z::t::nil)(add (add (var 0) (var 1))
-                                           (add (var 2) (var 3))) =
-        interp Z.add (x::y::z::t::nil)
+intros.
+change (interp Z Z.zero Z.add (x::y::z::t::nil)(add (add (var 0) (var 1))
+                                           (add (add (var 2) zero) (var 3))) =
+        interp Z Z.zero Z.add (x::y::z::t::nil)
               (add (add (var 0) (add (var 1) (var 2))) (var 3))).
-apply (norm_c2 Z.add_assoc).
+apply: normP Z.add_assoc Z.add_0_l Z.add_0_r _.
 reflexivity.
 Qed.
 
-From elpi Require Import elpi.
+(* This is for later *)
+Elpi Db monoid.db lp:{{ 
+  pred is_monoid
+    i:term, % type
+    o:term, % zero
+    o:term, % op
+    o:term, % assoc
+    o:term, % unit_l
+    o:term. % unit_r
+}}.
 
-Elpi Tactic reify.
+Elpi Tactic reify_list.
+Elpi Accumulate Db monoid.db.
 Elpi Accumulate lp:{{
 
+% 
 pred mem o:term, o:term, o:term.
 mem {{ lp:X :: lp:XS_ }} X {{0%nat}} :- !.
 mem {{ _ :: lp:XS }} X {{S lp:N}} :- mem XS X N.
@@ -72,172 +190,65 @@ pred close o:term.
 close {{ nil }} :- !.
 close {{ _ :: lp:XS }} :- close XS.
 
-pred quote i:term, i:term, o:term, o:term.
-quote GR (app [GR, T1, T2]) {{ add lp:R1 lp:R2 }} L :- !,
-  quote GR T1 R1 L,
-  quote GR T2 R2 L.
-quote _ T {{ var lp:R }} L :- mem L T R.
+pred quote i:term, i:term, i:term, o:term, o:term.
+quote Zero Op (app [Op, T1, T2]) {{ add lp:R1 lp:R2 }} L :- !,
+  quote Zero Op T1 R1 L,
+  quote Zero Op T2 R2 L.
+quote Zero _ Zero {{ zero }} _ :- !.
+quote _ _ T {{ var lp:R }} L :- mem L T R.
 
-solve [trm Op] [goal Ctx P {{ lp:A = lp:B }} _] _ :-
-  quote Op A AstA L,
-  quote Op B AstB L,
+solve [trm Zero, trm Op] [goal Ctx P {{ lp:A = lp:B }} _] _ :-
+  quote Zero Op A AstA L,
+  quote Zero Op B AstB L,
   close L,
   !,
-  Ty = {{ (interp lp:Op lp:L lp:AstA) = (interp lp:Op lp:L lp:AstB)}},
+  Ctx => coq.typecheck Zero T,
+  Ty = {{ (interp lp:T lp:Zero lp:Op lp:L lp:AstA) = (interp lp:T lp:Zero lp:Op lp:L lp:AstB)}},
   P = {{ (fun x : lp:Ty => x) _ }}.
+
+:name "error"
+solve _ _ _ :- coq.error "Not an equality".
 
 }}.
 Elpi Typecheck.
-Tactic Notation "reify_step" constr(x) := elpi reify (x).
+Tactic Notation "monoid_refl" constr(zero) constr(add) := elpi reify_list (zero) (add).
 
-
-Example axpypzpt2 (x : Z) : x = x.
-Proof.
-  reify_step Z.add.
-  now apply (norm_c2 Z.add_assoc); compute.
+Goal forall x y z t, (x + y) + (z + 0 + t) = x + (y + z) + t.
+Proof. 
+  intros.
+  monoid_refl 0 Z.add.
+  apply: normP Z.add_assoc Z.add_0_l Z.add_0_r _.
+  reflexivity.
 Qed.
 
-(* Now adding the reification phase. *)
+Elpi Accumulate monoid.db lp:{{
 
-Class Reify (op : Z -> Z -> Z) (t : lang) (l : list Z) (x : Z).
+  is_monoid {{ Z }} {{ 0 }} {{ Z.add }} {{ Z.add_assoc }} {{ Z.add_0_l }} {{ Z.add_0_r }}.
 
-Instance addRf op x y l e1 e2 {_ : Reify op e1 l x} {_ : Reify op e2 l y} :
-   Reify op (add e1 e2) l (op x y) | 1 := {}.
+}}.
 
-Class Nth (i : nat) (l : list Z) (e : Z).
+Elpi Accumulate reify_list lp:{{
 
-Instance nth0 t l : Nth 0 (t :: l) t | 0 := {}.
+:before "error"
+solve [] [G] GL :-
+  G = goal _ _ {{ @eq lp:T lp:A lp:B }} _,
+  std.assert! (is_monoid T Zero Op Assoc Ul Ur) "not a monoid",
+  quote Zero Op A AstA L,
+  quote Zero Op B AstB L,
+  close L,
+  !,
+  thenl [
+    refine {{ @normP lp:T lp:Zero lp:Op lp:L lp:AstA lp:AstB lp:Assoc lp:Ul lp:Ur _ }},
+    coq.ltac1.call "compute" [], % https://github.com/coq/coq/issues/10769
+    coq.ltac1.call "reflexivity" []
+  ] G GL.
 
-Instance nthS i t l t'
-   {_ : Nth i l t} : Nth (S i) (t' :: l) t | 2 := {}.
+}}.
+Elpi Typecheck.
+Tactic Notation "monoid_refl" := elpi reify_list.
 
-Instance varRf op e i l 
-  {_ : Nth i l e} : Reify op (var i) l e | 100 := {}.
-
-Class closed (l : list Z).
-
-Instance closed0 : closed nil := {}.
-
-Instance closed1 a l {_ : closed l} : closed (a :: l) := {}.
-
-Definition reify_trigger op (expr : lang) (lvar : list Z) (term : Z)
- {_ : Reify op expr lvar term} `{closed lvar} := (lvar, expr).
-
-Ltac reify_step_ltac op := time(
-match goal with |- ?u = ?v =>
-  match eval red in (reify_trigger op _ _ (op u v)) with
-    (?a, add ?b ?c) => change (interp op a b = interp op a c)
-  end
-end).
-
-Example axpypzpt23 x y z t : (x + y) + (z + t) = x + (y + z) + t.
-Proof.
-reify_step_ltac Z.add.
-now apply (norm_c2 Z.add_assoc); compute.
-Qed.
-
-(* Now adding the commutative property to the operator. *)
-
-Fixpoint lang_insert (x : nat) (t : lang) :=
-  match t with
-    add (var y) t' =>
-      if (x <=? y)%nat then add (var x) (add (var y) t')
-      else add (var y) (lang_insert x t')
-  | var y =>
-      if (x <=? y)%nat then add (var x) (var y)
-      else add (var y) (var x)
-  | _ => add (var x) t
-  end.
-
-Fixpoint lang_sort (t : lang) :=
-  match t with
-  | add (var x) t' => lang_insert x (lang_sort t')
-  | _ => t
-  end.
-
-Section comm_reflection_proofs.
-
-Variable op : Z -> Z -> Z.
-
-Hypotheses (op_assoc : forall a b c, op a (op b c) = op (op a b) c)
-  (op_comm : forall a b, op a b = op b a).
-
-Lemma lang_insert_c l x t :
-  interp op l (lang_insert x t) = interp op l (add (var x) t).
-Proof.
-induction t as [ j | [ j | t11 t12] _ t2 IH ]; simpl; auto;
-  case (x <=? j)%nat; simpl; auto.
-now rewrite IH; simpl; rewrite !op_assoc, (op_comm (_ x l 0)).
-Qed.
-
-Lemma lang_sort_c l t :
-  interp op l (lang_sort t) = interp op l t.
-Proof.
-induction t as [ i | [ j | t11 t12] _ t2 IH]; auto.
-now simpl; rewrite lang_insert_c; simpl; rewrite IH.
-Qed.
-
-Lemma lang_sort_c2 l t1 t2 :
-  lang_sort (norm t1) = lang_sort (norm t2) -> interp op l t1 = interp op l t2.
-Proof.
-intros nn; rewrite (norm_c _ op_assoc _ t1), (norm_c _ op_assoc _ t2).
-rewrite <- (lang_sort_c _ (norm t1)), <- (lang_sort_c _ (norm t2)).
-now apply f_equal.
-Qed.
-
-End comm_reflection_proofs.
-
-Arguments lang_sort_c2 {op}.
-
-Example cxpypz x y z : x + y + z = z + x + y.
-Proof.
-reify_step Z.add.
-apply (lang_sort_c2 Z.add_assoc Z.add_comm).
-compute.
-reflexivity.
-Qed.
-
-Example cxmymy x y : x * y * y = y * x * y.
-Proof.
-reify_step Z.mul.
-apply (lang_sort_c2 Z.mul_assoc Z.mul_comm).
-compute.
-reflexivity.
-Qed.
-
-Class comm_monoid (op : Z -> Z -> Z) :=
-  {op_assoc : forall x y z, op x (op y z) = op (op x y) z;
-   op_comm : forall x y, op x y = op y x}.
-
-Lemma lang_sort_c2' {op : Z -> Z -> Z} `{comm_monoid op} l t1 t2 :
-  lang_sort (norm t1) = lang_sort (norm t2) ->
-  interp op l t1 = interp op l t2.
-Proof.
-intros sn2; apply lang_sort_c2, sn2.
-  apply op_assoc.
-now apply op_comm.
-Qed.
-
-Example cxpypz2 x y z : x + y + z = z + x + y.
-Proof.
-reify_step Z.add.
-Fail apply lang_sort_c2'.
-Abort.
-
-Instance add_comm_monoid : comm_monoid Z.add :=
-  {op_assoc := Z.add_assoc; op_comm := Z.add_comm}.
-
-Instance mul_comm_monoid : comm_monoid Z.mul :=
-  {op_assoc := Z.mul_assoc; op_comm := Z.mul_comm}.
-
-Example cxpypz2 x y z : x + y + z = z + x + y.
-Proof.
-reify_step Z.add.
-now apply lang_sort_c2'.
-Qed.
-
-Example cxmymz2 x y z : x * y * z = z * x * y.
-Proof.
-reify_step Z.mul.
-now apply lang_sort_c2'.
+Goal forall x y z t, (x + y) + (z + 0 + t) = x + (y + z) + t.
+Proof. 
+  intros. 
+  monoid_refl.
 Qed.
